\documentclass[11pt, numbers=endperiod, parskip=half]{scrartcl}

\usepackage{amsmath}
\usepackage{color}
\usepackage{semantic}
\usepackage{soul}
\usepackage{pdflscape}

\title{Assignment 2}
\subtitle{COS30023 - Languages in Software Development}
\author{Daniel Parker - 971328X}

\date{\today}

\begin{document}
\maketitle

\section{Problem 1}
\subsection{Hoare Triple}
\begin{verbatim}
{a > 4, b = 7}
  x := b;
  y := a;
{a > 4, b = 7, x = 7, y > 4}
\end{verbatim}

\subsection{Rules}
%%%%%%%%%%%%%%%%%%%%%%%%%
%		  RULES         %
%%%%%%%%%%%%%%%%%%%%%%%%%
\inference[C = \textsuperscript{def} C.Target := C.Source : ]{true}{\{Q[C.Target \\\ C.Source]\} C \{Q\}}
\bigskip
\inference[C = \textsuperscript{def} C\textsubscript{1}; C\textsubscript{2} : ]{\{P\}C\textsubscript{1}\{R\} & \{R\}C\textsubscript{2}\{Q\}}{\{P\}C\textsubscript{1};C\textsubscript{2}\{Q\}}

\subsection{Proof}

\inference{\{ a > 4, b = 7 \} x := b \{R\} & \{R\} y := a \{ a > 4, b = 7, x = 7, y > 4 \} }{ \{ a > 4, b = 7 \} x := b; y := a; \{ a > 4, b = 7, x = 7, y > 4 \} }

\bigskip
\(\{R\} C_2: y := a; \{ a > 4, b = 7, x = 7, y > 4\}\)
\begin{flalign*}
\{R\} &= \{ a > 4, b = 7, x = 7, y > 4\}\lbrack y \backslash a \rbrack &\\
      &= \{ a > 4, b = 7, x = 7, a > 4\} \\
      &= \{ a > 4, b = 7, x = 7, \hbox{\st{a $>$ 4}}\} \\
\{R\} &= \{ a > 4, b = 7, x = 7\}
\end{flalign*}

\bigskip
\(\{ a > 4, b = 7\} C_1: x := b; \{R: a > 4, b = 7, x = 7\}\)
\begin{flalign*}
\{ a > 4, b = 7\}	&= \{ a > 4, b = 7, x = 7\}\lbrack x \backslash b \rbrack &\\
					&= \{ a > 4, b = 7, b = 7\} \\
					&= \{ a > 4, b = 7, \hbox{\st{b = 7}}\} \\
\{ a > 4, b = 7\}	&= \{ a > 4, b = 7\} \\
\end{flalign*}

\section{Problem 2}
\subsection{Hoare Triple}
\begin{verbatim}
{true}
  if x < 0 then val := -x; else val := x;
{val = abs(x)}
\end{verbatim}

\subsection{Rules}
\inference[C = \textsuperscript{def} if C.Test then C.Then else C.Else : ]{ \{ P \wedge C.Test \} C.Then \{ Q \} & \{ P \wedge \neg C.Test \} C.Else \{ Q \} }{ \{P\}C\{Q\} }
\bigskip
\inference{P => P' & \{P'\} C \{Q'\} & Q' => Q }{\{P\}C\{Q\}}

\subsection{Proof}
\inference{ \{true \wedge x < 0\} val := -x; \{ val = abs(x) \} & \{ true \wedge x \geq 0 \} val := x; \{ val = abs(x) \} }{ \{ true \}\ if\ x < 0\ then\ val := -x;\ else\ val := x; \{ val = abs(x) \} }

\subsubsection{Premise 1}
\inference{x < 0 => -x = abs(x) & \inference{true}{ \{ -x = abs(x) \} val := -x; \{ val = abs(x) \} } }{ \{ x < 0 \} val := -x; \{ val = abs(x) \} }

\subsubsection{Premise 2}
\inference{x \geq 0 => x = abs(x) & \inference{true}{ \{ x = abs(x) \} val := x; \{ val = abs(x) \} } }{ \{ x \geq 0 \} val := x; \{ val = abs(x) \} }

\setpremisesspace{1em}
\setpremisesend{0.5em}
\begin{landscape}
\subsubsection{Full Proof}
\inference{ \inference{x < 0 => -x = abs(x) & \inference{true}{ \{ -x = abs(x) \} val := -x; \{ val = abs(x) \} } }{ \{ x < 0 \wedge true \} val := -x; \{ val = abs(x) \} } & \inference{x \geq 0 => x = abs(x) & \inference{true}{ \{ x = abs(x) \} val := x; \{ val = abs(x) \} } }{ \{ x \geq 0 \wedge true \} val := x; \{ val = abs(x) \} } }{ \{ true \}\ if\ x < 0\ then\ val := -x;\ else\ val := x; \{ val = abs(x) \} }
\end{landscape}
\end{document}
